examples/archive/Monads.thy
@@ -605,7 +605,7 @@ next
 next
   case goal4 then show ?case    
        apply(erule_tac Q="None = (* FIXME to be shorten *) (case k b of None \<Rightarrow> None | Some S \<Rightarrow> let S' = (\<lambda>(x, y). h x y) ` S in if None \<in> S' then None else Some (\<Union>(the ` S')))" in contrapos_pp)
-       apply(erule_tac x="(aa,b)" and P="\<lambda> x. None \<noteq> split (\<lambda>out. k) x" in ballE)
+       apply(erule_tac x="(aa,b)" in ballE)
        apply(auto simp: aux Option.not_None_eq image_def split_def intro!: rev_bexI)
        done
 next 
